backend/Unusedglobproof.v
@@ -1160,10 +1160,10 @@ Local Transparent Mem.loadbytes.
   generalize (S1 NO). unfold Mem.loadbytes. destruct Mem.range_perm_dec; intros E1; inv E1.
   generalize (S2 NO). unfold Mem.loadbytes. destruct Mem.range_perm_dec; intros E2; inv E2.
   rewrite Z.add_0_r.
-  apply Mem_getN_forall2 with (p := 0) (n := nat_of_Z (init_data_list_size (gvar_init v))).
+  apply Mem_getN_forall2 with (p := 0) (n := Z.to_nat (init_data_list_size (gvar_init v))).
   rewrite H3, H4. apply bytes_of_init_inject. auto.
   omega.
-  rewrite nat_of_Z_eq by (apply init_data_list_size_pos). omega.
+  rewrite Z2Nat.id by (apply Z.ge_le; apply init_data_list_size_pos). omega.
 Qed.
 
 Lemma init_mem_inj_2:
